\begin{dmath*}
Pss = 1
\end{dmath*}
\begin{dmath*}
Rss = {Pss}_{t}\, \left(\frac{1}{{beta}}-\left(1-{delta}\right)\right)
\end{dmath*}
\begin{dmath*}
Wss = \left(1-{alpha}\right)\, {Pss}_{t}^{\frac{1}{1-{alpha}}}\, \left(\frac{{alpha}}{{Rss}_{t}}\right)^{\frac{{alpha}}{1-{alpha}}}
\end{dmath*}
\begin{dmath*}
Yss = \left(\frac{{Rss}_{t}}{{Rss}_{t}-{delta}\, {alpha}}\right)^{\frac{{sigma}}{{sigma}+{phi}}}\, \left(\left(1-{alpha}\right)^{\left(-{phi}\right)}\, \left(\frac{{Wss}_{t}}{{Pss}_{t}}\right)^{1+{phi}}\right)^{\frac{1}{{sigma}+{phi}}}
\end{dmath*}
\begin{dmath*}
Kss = {alpha}\, \frac{\frac{{Yss}_{t}}{{Rss}_{t}}}{{Pss}_{t}}
\end{dmath*}
\begin{dmath*}
Iss = {delta}\, {Kss}_{t}
\end{dmath*}
\begin{dmath*}
Css = {Yss}_{t}-{Iss}_{t}
\end{dmath*}
\begin{dmath*}
Lss = \left(1-{alpha}\right)\, \frac{\frac{{Yss}_{t}}{{Wss}_{t}}}{{Pss}_{t}}
\end{dmath*}
% Equation 1
\begin{dmath}
{sigma}\, {{C}}_{t}+{phi}\, {{L}}_{t}={{W}}_{t}
\end{dmath}
% Equation 2
\begin{dmath}
\frac{{sigma}}{{beta}}\, \left({{C}}_{t+1}-{{C}}_{t}\right)={Rss}_{t}\, {{R}}_{t+1}
\end{dmath}
% Equation 3
\begin{dmath}
{{K}}_{t}=\left(1-{delta}\right)\, {{K}}_{t-1}+{delta}\, {{I}}_{t}
\end{dmath}
% Equation 4
\begin{dmath}
{{Y}}_{t}={{A}}_{t}+{alpha}\, {{K}}_{t-1}+\left(1-{alpha}\right)\, {{L}}_{t}
\end{dmath}
% Equation 5
\begin{dmath}
{{R}}_{t}={{Y}}_{t}-{{K}}_{t-1}
\end{dmath}
% Equation 6
\begin{dmath}
{{W}}_{t}={{Y}}_{t}-{{L}}_{t}
\end{dmath}
% Equation 7
\begin{dmath}
{Yss}_{t}\, {{Y}}_{t}={{C}}_{t}\, {Css}_{t}+{Iss}_{t}\, {{I}}_{t}
\end{dmath}
% Equation 8
\begin{dmath}
{{A}}_{t}={rhoa}\, {{A}}_{t-1}+{e}_{t}
\end{dmath}
